make WeakestPrecondition.cmd complete wrt exec
by leaving the structurally recursive cases of cmd_body unchanged,
and defining the two non-structurally recursive cases (loop and call)
directly in terms of exec.
This seems to be the only approach that does not break proofs in
bedrock2Examples too badly.

bedrock2/src/bedrock2/WeakestPrecondition.v
@@ -1,12 +1,7 @@
 Require Import coqutil.Macros.subst coqutil.Macros.unique coqutil.Map.Interface coqutil.Map.OfListWord.
 Require Import Coq.ZArith.BinIntDef coqutil.Word.Interface coqutil.Word.Bitwidth.
 Require Import coqutil.dlet bedrock2.Syntax bedrock2.Semantics.
-
-Require Import coqutil.Map.Interface.
-Require coqutil.Map.SortedListString.
-
-#[export] Instance env: map.map String.string Syntax.func := SortedListString.map _.
-#[export] Instance env_ok: map.ok env := SortedListString.ok _.
+Require Import bedrock2.WP.
 
 Section WeakestPrecondition.
   Context {width: Z} {BW: Bitwidth width} {word: word.word width} {mem: map.map word Byte.byte}.
@@ -47,28 +42,6 @@ Section WeakestPrecondition.
     Fixpoint expr e := expr_body expr e.
   End WithMemAndLocals.
 
-  Ltac t :=
-    repeat match goal with
-      | |- forall _, _ => progress intros
-      | H: exists _, _ |- _ => destruct H
-      | H: and _ _ |- _ => destruct H
-      | H: eq _ ?y |- _ => subst y
-      | _ => progress cbn in *
-      end; eauto.
-
-  Lemma expr_sound: forall m l e mc post (H : expr m l e post),
-    exists v mc', Semantics.eval_expr m l e mc = Some (v, mc') /\ post v.
-  Proof.
-    induction e; t.
-    { destruct H. destruct H. eexists. eexists. rewrite H. eauto. }
-    { eapply IHe in H; t. cbv [load] in H0; t. rewrite H. rewrite H0. eauto. }
-    { eapply IHe in H; t. cbv [load] in H0; t. rewrite H. rewrite H0. eauto. }
-    { eapply IHe1 in H; t. eapply IHe2 in H0; t. rewrite H, H0; eauto. }
-    { eapply IHe1 in H; t. rewrite H. Tactics.destruct_one_match.
-      { eapply IHe3 in H0; t. }
-      { eapply IHe2 in H0; t. } }
-  Qed.
-
   Section WithF.
     Context {A B} (f: A -> (B -> Prop) -> Prop).
     Definition list_map_body rec (xs : list A) (post : list B -> Prop) : Prop :=
@@ -82,210 +55,81 @@ Section WeakestPrecondition.
     Fixpoint list_map xs := list_map_body list_map xs.
   End WithF.
 
-  Lemma exprs_sound : forall m l args mc P,
-      list_map (expr m l) args P ->
-      exists x mc', Semantics.evaluate_call_args_log m l args mc = Some (x, mc') /\ P x.
-  Proof.
-    induction args; cbn; repeat (subst; t).
-    unfold Semantics.eval_expr in *.
-    eapply expr_sound in H; t; rewrite H.
-    eapply IHargs in H0; t; rewrite H0.
-    eauto.
-  Qed.
-
-  Lemma getmany_sound: forall a l P,
-      list_map (get l) a P -> exists vs, map.getmany_of_list l a = Some vs /\ P vs.
-  Proof.
-    cbv [map.getmany_of_list].
-    induction a; cbn; repeat (subst; t).
-    cbv [get] in H; t.
-    epose proof (IHa _ _ H0); clear IHa; t.
-    rewrite H. erewrite H1. eexists; split; eauto.
-  Qed.
-
-  Definition dexpr m l e v := expr m l e (eq v).
-  Definition dexprs m l es vs := list_map (expr m l) es (eq vs).
-
-  Section WithFunctionEnv.
+  Section WithFunctions.
     Context (e: env).
-
-    Inductive cmd (c : Syntax.cmd) (t : trace) (m : mem) (l : locals)
-      (post : (trace -> mem -> locals -> Prop)) : Prop :=
-    | mk_cmd (_ : forall mc, exec e c t m l mc (fun t' m' l' mc' => post t' m' l')).
-
-    Lemma invert_cmd: forall c t m l post,
-        cmd c t m l post ->
-        forall mc, exec e c t m l mc (fun t' m' l' mc' => post t' m' l').
-    Proof. intros. inversion H. apply H0. Qed.
-
-    Definition func '(innames, outnames, c) (t : trace) (m : mem) (args : list word)
-      (post : trace -> mem -> list word -> Prop) :=
-      exists l, map.of_list_zip innames args = Some l /\
-      cmd c t m l (fun t m l =>
-        list_map (get l) outnames (fun rets =>
-        post t m rets)).
-
-    Definition call (fname: String.string) :=
-      match map.get e fname with
-      | Some fimpl => func fimpl
-      | None => fun _ _ _ _ => False
-      end.
-
-    Implicit Type post : trace -> mem -> locals -> Prop.
-
-    Ltac step :=
-      match reverse goal with
-      | H: _ /\ _ |- _ => destruct H
-      | H: exists x, _ |- _ => let n := fresh x in destruct H as [n H]
-      | |- _ => progress unfold dlet, dexpr, store in *
-      | H: cmd _ _ _ _ _ |- _ => pose proof (invert_cmd _ _ _ _ _ H); clear H
-      | |- _ => constructor
-      | |- _ => assumption
-      | H: forall _: MetricLogging.MetricLog, _ |- _ => apply H
-      | |- _ => progress intros
-      | |- _ => progress subst
-      (* creates an evar for metrics, therefore needs to be applied from top to bottom,
-         so we need `match reverse` instead of `match` *)
-      | H: expr _ _ _ _ |- _ => eapply expr_sound in H
-      | |- _ => solve [econstructor; eauto]
-      end.
-    Ltac tac := repeat step.
-
-    Lemma wp_skip: forall t m l post, post t m l -> cmd cmd.skip t m l post.
-    Proof. tac. Qed.
-
-    Lemma wp_set: forall x ev t m l post,
-        (exists v, dexpr m l ev v /\
+    Definition dexpr m l e v := expr m l e (eq v).
+    Definition dexprs m l es vs := list_map (expr m l) es (eq vs).
+    (* All cases except cmd.while and cmd.call can be denoted by structural recursion
+       over the syntax.
+       For cmd.while and cmd.call, we fall back to the operational semantics *)
+    Definition cmd_body (rec:_->_->_->_->_->Prop) (c : cmd) (t : trace) (m : mem) (l : locals)
+             (post : trace -> mem -> locals -> Prop) : Prop :=
+      (* give value of each pure expression when stating its subproof *)
+      match c with
+      | cmd.skip => post t m l
+      | cmd.set x ev =>
+        exists v, dexpr m l ev v /\
         dlet! l := map.put l x v in
-        post t m l) ->
-        cmd (cmd.set x ev) t m l post.
-    Proof. tac. Qed.
-
-    Lemma wp_unset: forall x t m l post,
-        (dlet! l := map.remove l x in
-         post t m l) ->
-        cmd (cmd.unset x) t m l post.
-    Proof. tac. Qed.
-
-    Lemma wp_store: forall sz ea ev t m l post,
-       (exists a, dexpr m l ea a /\
+        post t m l
+      | cmd.unset x =>
+        dlet! l := map.remove l x in
+        post t m l
+      | cmd.store sz ea ev =>
+        exists a, dexpr m l ea a /\
         exists v, dexpr m l ev v /\
         store sz m a v (fun m =>
-        post t m l)) ->
-       cmd (cmd.store sz ea ev) t m l post.
-    Proof. tac. Qed.
-
-    Lemma wp_stackalloc: forall x n c t m l post,
-        (Z.modulo n (bytes_per_word width) = 0 /\
+        post t m l)
+      | cmd.stackalloc x n c =>
+        Z.modulo n (bytes_per_word width) = 0 /\
         forall a mStack mCombined,
           anybytes a n mStack -> map.split mCombined m mStack ->
           dlet! l := map.put l x a in
-          cmd c t mCombined l (fun t' mCombined' l' =>
+          rec c t mCombined l (fun t' mCombined' l' =>
           exists m' mStack',
           anybytes a n mStack' /\ map.split mCombined' m' mStack' /\
-          post t' m' l')) ->
-          cmd (cmd.stackalloc x n c) t m l post.
-    Proof. tac. specialize H0 with (1 := H1) (2 := H2). tac. Qed.
-
-    Lemma wp_cond: forall br ct cf t m l post,
-        (exists v, dexpr m l br v /\
-        (word.unsigned v <> 0%Z -> cmd ct t m l post) /\
-        (word.unsigned v = 0%Z -> cmd cf t m l post)) ->
-        cmd (cmd.cond br ct cf) t m l post.
-    Proof.
-      tac. destr.destr (Z.eqb (word.unsigned v0) 0).
-      - specialize H1 with (1 := E). tac.
-      - specialize H0 with (1 := E). tac.
-    Qed.
-
-    Lemma wp_seq: forall c1 c2 t m l post,
-        cmd c1 t m l (fun t m l => cmd c2 t m l post) ->
-        cmd (cmd.seq c1 c2) t m l post.
-    Proof.
-      tac. eapply exec.weaken.
-      { econstructor. 1: eapply H0. tac. }
-      tac.
-    Qed.
-
-    Lemma wp_while: forall e c t m l post,
-       (exists measure (lt:measure->measure->Prop) (inv:measure->trace->mem->locals->Prop),
-        Coq.Init.Wf.well_founded lt /\
-        (exists v, inv v t m l) /\
-        (forall v t m l, inv v t m l ->
-          exists b, dexpr m l e b /\
-          (word.unsigned b <> 0%Z -> cmd c t m l (fun t' m l =>
-            exists v', inv v' t' m l /\ lt v' v)) /\
-          (word.unsigned b = 0%Z -> post t m l))) ->
-       cmd (cmd.while e c) t m l post.
-    Proof.
-      intros. destruct H as (measure & lt & inv & Hwf & HInit & Hbody).
-      destruct HInit as (v0 & HInit).
-      econstructor. intros.
-      revert t m l mc HInit. pattern v0. revert v0.
-      eapply (well_founded_ind Hwf). intros.
-      specialize Hbody with (1 := HInit). destruct Hbody as (b & Hb & Ht & Hf).
-      eapply expr_sound in Hb. destruct Hb as (b' & mc' & Hb & ?). subst b'.
-      destr.destr (Z.eqb (word.unsigned b) 0).
-      - specialize Hf with (1 := E). eapply exec.while_false; eassumption.
-      - specialize Ht with (1 := E). inversion Ht. clear Ht.
-        eapply exec.while_true; eauto.
-        cbv beta. intros * (v' & HInv & HLt). eauto.
-    Qed.
-
-    Lemma wp_call: forall binds fname arges t m l post,
-       (exists args, dexprs m l arges args /\
-        call fname t m args (fun t m rets =>
+          post t' m' l')
+      | cmd.cond br ct cf =>
+        exists v, dexpr m l br v /\
+        (word.unsigned v <> 0%Z -> rec ct t m l post) /\
+        (word.unsigned v = 0%Z -> rec cf t m l post)
+      | cmd.seq c1 c2 =>
+        rec c1 t m l (fun t m l => rec c2 t m l post)
+      | cmd.while _ _ => wp_cmd e c t m l post
+      | cmd.call binds fname arges =>
+        exists args, dexprs m l arges args /\
+        wp_call e fname t m args (fun t m rets =>
           exists l', map.putmany_of_list_zip binds rets l = Some l' /\
-          post t m l')) ->
-       cmd (cmd.call binds fname arges) t m l post.
-    Proof.
-      tac.
-      unfold dexprs in *.
-      eapply exprs_sound in H. destruct H as (argvs & mc' & HEv & ?). subst argvs.
-      unfold call in *.
-      Tactics.destruct_one_match_hyp. 2: contradiction.
-      unfold func in *.
-      destruct f as ((argnames & retnames) & fbody).
-      destruct H0 as (l1 & Hl1 & Hbody).
-      inversion Hbody. clear Hbody. rename H into Hbody.
-      eapply exec.call; eauto.
-      cbv beta. intros. eapply getmany_sound. assumption.
-    Qed.
-
-    Lemma wp_interact: forall binds action arges t m l post,
-       (exists args, dexprs m l arges args /\
+          post t m l')
+      | cmd.interact binds action arges =>
+        exists args, dexprs m l arges args /\
         exists mKeep mGive, map.split m mKeep mGive /\
         ext_spec t mGive action args (fun mReceive rets =>
           exists l', map.putmany_of_list_zip binds rets l = Some l' /\
           forall m', map.split m' mKeep mReceive ->
-          post (cons ((mGive, action, args), (mReceive, rets)) t) m' l')) ->
-       cmd (cmd.interact binds action arges) t m l post.
-    Proof.
-      tac.
-      eapply exprs_sound in H. destruct H as (argvs & mc' & HEv & ?). subst argvs.
-      tac.
-    Qed.
-  End WithFunctionEnv.
+          post (cons ((mGive, action, args), (mReceive, rets)) t) m' l')
+      end.
+    Fixpoint cmd c := cmd_body cmd c.
+  End WithFunctions.
+
+  Definition func call '(innames, outnames, c) (t : trace) (m : mem) (args : list word) (post : trace -> mem -> list word -> Prop) :=
+      exists l, map.of_list_zip innames args = Some l /\
+      cmd call c t m l (fun t m l =>
+        list_map (get l) outnames (fun rets =>
+        post t m rets)).
 End WeakestPrecondition.
+Notation call := wp_call.
 
-Ltac apply_rule_for_command c :=
-  lazymatch c with
-  | cmd.skip => eapply wp_skip
-  | cmd.set ?x ?ev => eapply wp_set
-  | cmd.unset ?x => eapply wp_unset
-  | cmd.store ?sz ?ea ?ev => eapply wp_store
-  | cmd.stackalloc ?x ?n ?c => eapply wp_stackalloc
-  | cmd.cond ?br ?ct ?cf => eapply wp_cond
-  | cmd.seq ?c1 ?c2 => eapply wp_seq
-  | cmd.while ?e ?c => eapply wp_while
-  | cmd.call ?binds ?fname ?arges => eapply wp_call
-  | cmd.interact ?binds ?action ?arges => eapply wp_interact
+Ltac unfold1_cmd e :=
+  lazymatch e with
+    @cmd ?width ?BW ?word ?mem ?locals ?ext_spec ?CA ?c ?t ?m ?l ?post =>
+    let c := eval hnf in c in
+    constr:(@cmd_body width BW word mem locals ext_spec CA
+                      (@cmd width BW word mem locals ext_spec CA) c t m l post)
   end.
-
 Ltac unfold1_cmd_goal :=
-  lazymatch goal with
-  | |- cmd _ ?c _ _ _ ?post => let c := eval hnf in c in apply_rule_for_command c
-  end.
+  let G := lazymatch goal with |- ?G => G end in
+  let G := unfold1_cmd G in
+  change G.
 
 Ltac unfold1_expr e :=
   lazymatch e with
