bedrock2/src/bedrock2/WP.v
@@ -1,0 +1,122 @@
+Require Import Coq.ZArith.ZArith.
+Require Import coqutil.Map.Interface.
+Require coqutil.Map.SortedListString.
+Require Import coqutil.Word.Interface coqutil.Word.Bitwidth.
+Require Import bedrock2.Syntax bedrock2.Semantics.
+
+#[export] Instance env: map.map String.string Syntax.func := SortedListString.map _.
+#[export] Instance env_ok: map.ok env := SortedListString.ok _.
+
+(* We want to make the definitions opaque to `hnf` (unfolds any definition, so a plain
+   definition doesn't work) and to `repeat split` (applies constructors of all
+   1-constructor inductives, so a 1-constructor inductive wrapping exec doesn't
+   work). *)
+Module Type WP_Sig.
+  Section WithParams.
+    Context {width: Z} {BW: Bitwidth width} {word: word.word width}
+      {mem: map.map word Byte.byte}
+      {locals: map.map String.string word}.
+
+    Parameter wp_cmd : forall {ext_spec: ExtSpec} (e: env),
+        Syntax.cmd -> trace -> mem -> locals ->
+        (trace -> mem -> locals -> Prop) -> Prop.
+    Parameter mk_wp_cmd : forall {ext_spec: ExtSpec} (e: env) c t m l post,
+        (forall mc, exec e c t m l mc (fun t' m' l' mc' => post t' m' l')) ->
+        wp_cmd e c t m l post.
+    Parameter invert_wp_cmd: forall {ext_spec: ExtSpec} [e c t m l post],
+        wp_cmd e c t m l post ->
+        forall mc, exec e c t m l mc (fun t' m' l' mc' => post t' m' l').
+
+    Parameter wp_call : forall {locals: map.map String.string word} {ext_spec: ExtSpec},
+        env -> String.string -> trace -> mem -> list word ->
+        (trace -> mem -> list word -> Prop) -> Prop.
+    Parameter mk_wp_call :
+      forall {ext_spec: ExtSpec} (e: env) fname argnames retnames body t m l args post,
+        map.get e fname = Some (argnames, retnames, body) ->
+        map.of_list_zip argnames args = Some l ->
+        wp_cmd e body t m l (fun t' m' l' => exists rets,
+          map.getmany_of_list l' retnames = Some rets /\ post t' m' rets) ->
+        wp_call e fname t m args post.
+    Parameter invert_wp_call : forall {ext_spec: ExtSpec} (e: env) fname t m args post,
+        wp_call e fname t m args post ->
+        exists argnames retnames body l,
+          map.get e fname = Some (argnames, retnames, body) /\
+          map.of_list_zip argnames args = Some l /\
+          wp_cmd e body t m l (fun t' m' l' => exists rets,
+            map.getmany_of_list l' retnames = Some rets /\ post t' m' rets).
+  End WithParams.
+End WP_Sig.
+
+Module Export WP_Impl : WP_Sig.
+  Section WithParams.
+    Context {width: Z} {BW: Bitwidth width} {word: word.word width}
+      {mem: map.map word Byte.byte}
+      {locals: map.map String.string word}
+      {ext_spec: ExtSpec}
+      (e: env).
+
+    Definition wp_cmd (c : Syntax.cmd) (t : trace) (m : mem) (l : locals)
+      (post : (trace -> mem -> locals -> Prop)) : Prop :=
+      (forall mc, exec e c t m l mc (fun t' m' l' mc' => post t' m' l')).
+
+    Lemma mk_wp_cmd c t m l post:
+      (forall mc, exec e c t m l mc (fun t' m' l' mc' => post t' m' l')) ->
+      wp_cmd c t m l post.
+    Proof. exact id. Qed.
+
+    Lemma invert_wp_cmd c t m l post:
+        wp_cmd c t m l post ->
+        forall mc, exec e c t m l mc (fun t' m' l' mc' => post t' m' l').
+    Proof. exact id. Qed.
+
+    Definition wp_call fname t m args post :=
+        exists argnames retnames body l,
+          map.get e fname = Some (argnames, retnames, body) /\
+          map.of_list_zip argnames args = Some l /\
+          wp_cmd body t m l (fun t' m' l' => exists rets,
+            map.getmany_of_list l' retnames = Some rets /\ post t' m' rets).
+
+    Lemma mk_wp_call: forall fname argnames retnames body t m l args post,
+        map.get e fname = Some (argnames, retnames, body) ->
+        map.of_list_zip argnames args = Some l ->
+        wp_cmd body t m l (fun t' m' l' => exists rets,
+          map.getmany_of_list l' retnames = Some rets /\ post t' m' rets) ->
+        wp_call fname t m args post.
+    Proof. intros. unfold wp_call. eauto 8. Qed.
+
+    Lemma invert_wp_call fname t m args post:
+        wp_call fname t m args post ->
+        exists argnames retnames body l,
+          map.get e fname = Some (argnames, retnames, body) /\
+          map.of_list_zip argnames args = Some l /\
+          wp_cmd body t m l (fun t' m' l' => exists rets,
+            map.getmany_of_list l' retnames = Some rets /\ post t' m' rets).
+    Proof. exact id. Qed.
+  End WithParams.
+End WP_Impl.
+
+Section WithParams.
+  Context {width: Z} {BW: Bitwidth width} {word: word.word width}
+    {mem: map.map word Byte.byte}
+    {locals: map.map String.string word}
+    {ext_spec: ExtSpec}
+    (e: env).
+
+  Lemma weaken_wp_cmd: forall c t m l (post1 post2: trace -> mem -> locals -> Prop),
+      (forall t' m' l', post1 t' m' l' -> post2 t' m' l') ->
+      wp_cmd e t m l c post1 -> wp_cmd e t m l c post2.
+  Proof.
+    intros. eapply mk_wp_cmd. intros. eapply invert_wp_cmd in H0.
+    eapply exec.weaken. 1: eassumption. eauto.
+  Qed.
+
+  Lemma weaken_wp_call: forall f t m args (post1 post2: trace -> mem -> list word -> Prop),
+      (forall t' m' rets, post1 t' m' rets -> post2 t' m' rets) ->
+      wp_call e f t m args post1 -> wp_call e f t m args post2.
+  Proof.
+    intros. eapply invert_wp_call in H0. firstorder idtac.
+    eapply mk_wp_call; eauto.
+    eapply weaken_wp_cmd. 2: eassumption. firstorder eauto.
+  Qed.
+
+End WithParams.
